added definitions

bst.v
@@ -29,3 +29,49 @@ Fixpoint bst (T : tree) : Prop :=
   | leaf => True
   | node lt k rt => (bst lt) /\ (bst rt) /\ (lessTree lt k) /\ (grtTree rt k)
 end.
+
+(* Insert function for a binary search tree *)
+Fixpoint insert (n : nat) (T : tree) : tree :=
+  match T with
+  | leaf => (node leaf n leaf)
+  | node lt k rt => match (compare k n) with 
+      | Eq => T
+      | Lt => (node lt k (insert n rt))
+      | Gt => (node (insert n lt) k rt)
+  end
+end.
+
+(* Transform a regular binary tree into a list *)
+Fixpoint treeToList (T : tree) : list nat :=
+  match T with
+  | leaf => nil
+  | node lt k rt => cons k ((treeToList lt) ++ (treeToList rt))
+end.
+
+(* Transforms a list into a BST *)
+Fixpoint listToBST (L : list nat) : tree :=
+  match L with
+  | nil => leaf
+  | cons n ns => (insert n (listToBST ns))
+end.
+
+(* Transforms a tree into a BST *)
+Definition sort (T : tree) : tree := listToBST(treeToList T).
+
+(* Checks that an element occurs in a tree *)
+Fixpoint occurs (n : nat) (T : tree) : Prop :=
+  match T with
+  | leaf => False
+  | node lt k rt => (k = n) \/ (occurs n lt) \/ (occurs n rt)
+end.
+
+(* Proofs *)
+Theorem insertBST : forall t : tree, forall n : nat, bst t -> bst (insert n t).
+
+Theorem sortPreservesBST : forall t : tree, bst (sort t).
+
+Theorem occursBST : forall n : nat, forall t : tree, occurs n t <-> occurs n (sort t).
+
+
+
+
